update

Jrlean/Coc/Term.lean
@@ -12,18 +12,24 @@ namespace Jrlean.Coc
 public section
 
 /-- A term in the Calculus of Constructions. -/
-inductive Term [VarKind] : Type where
+@[grind]
+inductive Term {varKind : VarKind} : Type where
   /-- The type of propositions. -/
   | prop : Term
   /-- The type of types, except itself. -/
   | type : Term
   /-- A variable. -/
-  | var (v : Var) : Term
+  | var (v : Var') : Term
   /-- An application of a function to an argument. -/
-  | app (f : Term) (a : Term) : Term
+  | app (f : @Term varKind) (a : @Term varKind) : Term
   /-- Declares a binder from some variable of some type to a body. -/
-  | binder (k : BinderKind) (x : VarDecl) (ty : Term) (body : Term) : Term
+  | binder (k : BinderKind) (x : VarDecl') (ty : @Term varKind) (body : @Term varKind) : Term
   deriving DecidableEq, Inhabited, Hashable
 
-@[match_pattern] abbrev Term.lam [VarKind] := Term.binder (λ)
-@[match_pattern] abbrev Term.pi [VarKind]  := Term.binder (Π)
+/-- A version of `Term` that infers the variable kind via type-class inference. -/
+abbrev Term' [varKind : VarKind] := @Term varKind
+
+variable {varKind : VarKind}
+
+@[match_pattern] abbrev Term.lam := @Term.binder varKind (λ)
+@[match_pattern] abbrev Term.pi  := @Term.binder varKind (Π)
