Jrlean/Coc/TermNotation.lean
@@ -1,10 +1,17 @@
 module
 
 public import Jrlean.Coc.Term
+public import Jrlean.Coc.VarConversions
 public meta import Jrlean.Coc.BinderKindNotation
+public meta import Jrlean.Coe
+
+import Lean
+import Jrlean.Of
 
 open Lean (mkIdent quote)
 open Lean.PrettyPrinter (Unexpander)
+
+open Jrlean
 
 namespace Jrlean.Coc
 
@@ -12,10 +19,9 @@ public section
 
 variable {varKind : VarKind}
 
--- These allow us to write just `prop` and `type`, and they also infer the variable kind from the
--- types instead of from the context.
-public abbrev prop : Term := Term.prop
-public abbrev type : Term := Term.type
+-- These allow us to write just `prop` and `type`.
+@[match_pattern] public abbrev prop : Term' := Term.prop
+@[match_pattern] public abbrev type : Term' := Term.type
 -- These make the notation appear colored! ~^-^~
 notation "prop" => prop
 notation "type" => type
@@ -23,38 +29,44 @@ notation "type" => type
 @[app_unexpander Term.prop] meta def Term.prop.unexpander : Unexpander | _ => ``(prop)
 @[app_unexpander Term.type] meta def Term.type.unexpander : Unexpander | _ => ``(type)
 
--- Write applications as `f a`
-instance : CoeFun Term (fun _ => Term → Term) where
-  coe t := t.app
+-- Write applications as `f a`.
+-- Also allow us to treat things that convert to terms as applications.
+instance : CoeFun Term' fun _ => Term' → Term' where coe t := t.app
+-- instance : CoeFun Var' fun _ => Term' → Term' where coe t := (Term.var t).app
+instance {α} [CoeHOTC α Term'] : CoeFun α fun _ => Term' → Term' where
+  coe a := Term.app a
+-- instance : CoeFun Lean.Name fun _ => @Term .named → @Term .named where
+--   coe t := @Term.app .named (@Term.var .named t)
 @[app_unexpander app] meta def Term.app.unexpander : Unexpander
   | `(Term.app $f $a) => ``($f $a)
   | _ => throw ()
 
+#guard_expr (fun (f a : Term') => f a) = (fun (f a : Term') => f.app a)
+
 -- λ x : ty. body
-macro:arg k:binderKind ws x:ident " : " ty:term:max " . " body:term:min : term => do
-  ``(@Term.binder VarKind.named $k:term $(quote x.getId) $ty $body)
+macro:arg k:binderKind ws x:term:max " : " ty:term:max " . " body:term:min : term => do
+  ``(Term.binder $k:term $x $ty $body)
 @[app_unexpander binder] meta def Term.binder.unexpander : Unexpander
-  | `(Term.binder $k $x:name $ty $body) =>
+  | `(Term.binder $k $x $ty $body) =>
     match k with
-    | `(λ) => `(λ $(mkIdent x.getName) : $ty . $body)
-    | `(Π) => `(Π $(mkIdent x.getName) : $ty . $body)
+    | `(λ) => `(λ $x : $ty . $body)
+    | `(Π) => `(Π $x : $ty . $body)
     | _ => throw ()
   | _ => throw ()
 
--- var x or var `x or var 12
-public abbrev var := Term.var
-notation:arg "var " x:max => var x
-macro "var " x:ident : term => `(@Term.var .named ($(quote x.getId), 0))
-macro "var " n:num : term => `(@Term.var .deBruijn $n)
-@[app_unexpander Term.var] meta def Term.var.unexpander : Unexpander
-  | `(Term.var ($a:name, 0)) => `(var $(mkIdent a.getName):ident)
-  | `(Term.var $n:num) => `(var $n:num)
-  | `(Term.var $a) => `(var $a:term)
+-- `x or 12
+-- We can already write these as `Var` via coersions defined in `VarConversions.lean`. Just need to
+-- define coersions to terms.
+instance : CoeOut Var' Term' where coe := .var
+instance : Coe    Var' Term' where coe := .var
+public abbrev var : @Var varKind → @Term varKind := Term.var
+@[app_unexpander var] meta def Term.var.unexpander : Unexpander
+  | `(Term.var $v) => ``($v)
   | _ => throw ()
 
-
-/-- info: var x -/ #guard_msgs in #reduce var x
-/-- info: var x -/ #guard_msgs in #reduce @Term.var .named (`x, 0)
-/-- info: var (`x, 12) -/ #guard_msgs in #reduce @Term.var .named (`x, 12)
-/-- info: Π x : type . (var f) var x -/ #guard_msgs in
-#reduce Π x : (@Term.type .named) . (var f) var (`x, 0)
+/-- info: `x -/ #guard_msgs in #reduce (`x : @Term .named)
+/-- info: `x -/ #guard_msgs in #reduce @Term.var .named ⟨`x, 0⟩
+/-- info: ⟨`x, 12⟩ -/ #guard_msgs in #reduce @Term.var .named ⟨`x, 12⟩
+/-- info: Π `x : type . `f `x -/ #guard_msgs in #reduce Π `x : (@Term.type .named) . `f `x
+/-- info: Π `x : type . `f `x -/ #guard_msgs in #reduce Π `x : type . `f `x
+/-- info: λ `x : type . `f `x -/ #guard_msgs in #reduce λ `x : type . `f `x
