Jrlean.lean
@@ -20,4 +20,5 @@ public import Jrlean.DReader
 public import Jrlean.DependentState
 public import Jrlean.C
 public import Jrlean.Effect
+public import Jrlean.GetElemLater
 public import Jrlean.Coc
