Jrlean/Coc.lean
@@ -5,10 +5,24 @@ public import Jrlean.Coc.VarDecl
 public import Jrlean.Coc.Var
 public import Jrlean.Coc.VarConversions
 
+public import Jrlean.Coc.Offseting
+public import Jrlean.Coc.VarOffseting
+public import Jrlean.Coc.VarOffsetingLemmas
+public import Jrlean.Coc.TermOffseting
+public import Jrlean.Coc.TermOffsetingLemmas
+
 public import Jrlean.Coc.BinderKind
 public import Jrlean.Coc.BinderKindNotation
 public import Jrlean.Coc.Term
 public import Jrlean.Coc.TermNotation
+public import Jrlean.Coc.Sort
+
+public import Jrlean.Coc.VarSubst
+public import Jrlean.Coc.TermFreeVars
+public import Jrlean.Coc.Subst
+public import Jrlean.Coc.SubstLemmas
+
+public import Jrlean.Coc.BetaReducesTo
 
 /-!
 "CoC" stands for "Calculus of Constructions". It is an extension to the standard lambda calculus
@@ -19,4 +33,12 @@ with named identifiers.
 Everything is defined in the `Coc` namespace.
 
 In this module, the word `lambda` is sometimes written as `lam`.
+
+## Offseting
+
+Variables are defined either as de Bruijn indices or as named identifiers. Both representations are
+dependent on context, and need to be adjusted when the context changes. We call this offseting.
+A variable needs to be "offset in" by some variable when moved into a binder, and needs to be
+"offset out" by some variable declaration when moved out of it.
+An entire term can be offset in or out by a variable declaration as well.
 -/
