Jrlean/Coc/BetaReducesTo.lean
@@ -1,0 +1,46 @@
+module
+
+public import Jrlean.Coc.Term
+public import Jrlean.Coc.Subst
+
+import Jrlean.Coc.TermNotation
+import Jrlean.Coc.VarConversions
+import Jrlean.SetTactic
+
+public import Jrlean.Relation
+
+namespace Jrlean.Coc
+
+variable {varKind : VarKind}
+
+@[grind]
+public inductive Term.BetaReducesTo : Relation Term' Term' where
+  /-- A redex is a term that has a head as written here, and hence is reducible. -/
+  | redex {x a ty body} : ((λ x : ty . body) a).BetaReducesTo body[x:=a]
+  | reduceFunc {f g a : Term} : f.BetaReducesTo g → (f a).BetaReducesTo (g a)
+  | reduceArg {a b f : Term} : a.BetaReducesTo b → (f a).BetaReducesTo (f b)
+  | reduceBinderType {k x ty ty' body}
+    : ty.BetaReducesTo ty' → (binder k x ty body).BetaReducesTo (binder k x ty' body)
+  | reduceBinderBody {k x ty body body'}
+    : body.BetaReducesTo body' → (binder k x ty body).BetaReducesTo (binder k x ty body')
+
+-- Terms
+variable {a b c d e f g : Term}
+variable {t t' : Term}
+variable {ty ty' body body' : Term}
+-- Variables
+variable {x y z : VarDecl}
+-- Binder kind
+variable {k k' : BinderKind}
+
+
+theorem Term.betaReducesTo_prop
+(h_prop : t.BetaReducesTo prop)
+: (∃ x ty a, t = (λ x : ty . prop) a) ∨ (∃ x ty, t = (λ x : ty . x) prop) := by
+  -- Call the rhs t' so we can use elimination
+  set t' := prop with h_t'
+  cases h_prop
+  -- Redex!
+  case redex x a ty body =>
+    sorry
+
