Jrlean/Coc/Offseting.lean
@@ -1,0 +1,21 @@
+module
+
+import Init.Notation
+public import Jrlean.Coc.Var
+
+namespace Jrlean.Coc
+
+public class Offset (varKind : VarKind) (α : Type) where
+  offsetIn : α → Var' → α
+  offsetOut : α → Var' → Option α
+
+infix:arg "↑" => Offset.offsetIn
+infix:arg "↓" => Offset.offsetOut
+
+/--
+info:
+fun {varKind} [Offset varKind Var'] a b => (a↓b).get! : {varKind : VarKind} → [Offset varKind Var']
+→ Var' → Var' → Var'
+-/
+#guard_msgs in
+#check fun {varKind : VarKind} [Offset varKind Var'] (a b : Var') => Option.get! a↓b
