Jrlean/Coc/Subst.lean
@@ -1,0 +1,28 @@
+module
+
+public import Jrlean.Coc.VarSubst
+public import Jrlean.Coc.Term
+public import Jrlean.Coc.TermNotation
+
+import Jrlean.Of
+import Jrlean.Coe
+
+namespace Jrlean.Coc
+
+variable {varKind : VarKind}
+
+/-- t[x:=r] -/
+@[expose]
+public def Term.subst (t : Term') (x : Var') (r : Term') : Term' :=
+  match t with
+  | type => type
+  | prop => prop
+  | .var y => y.subst x r
+  | .app f a => (f.subst x r) (a.subst x r)
+  | .binder k yDecl ty body =>
+    let y := yDecl.toVar
+    binder k yDecl
+    of ty.subst x r
+    of body.subst y (x ↑ y)
+
+notation:max x "[" y ":=" r "]" => Term.subst x y r
