Jrlean/Coc/SubstLemmas.lean
@@ -1,0 +1,152 @@
+module
+
+public import Jrlean.Coc.Subst
+public import Jrlean.Coc.Sort
+public import Jrlean.Coc.VarOffseting
+public import Jrlean.Coc.TermOffseting
+public import Jrlean.Coc.TermFreeVars
+
+import Jrlean.Coc.VarOffsetingLemmas
+import Jrlean.Coc.TermOffsetingLemmas
+
+import Jrlean.Assumption
+import Jrlean.ByContra
+import Jrlean.SetTactic
+
+namespace Jrlean.Coc
+
+public section
+
+variable {varKind : VarKind}
+variable {a b c : Term'}
+variable {s : Term'} [IsSort s]
+variable {x : Var}
+
+@[grind =, simp]
+theorem var_subst_eq
+{x : Var'} {r}
+: x.subst x r = r := by
+  simp only [Var.subst, Var.offsetOut.simp_notation, Var.offsetOut]
+  grind only [= Var.offsetOutDeBruijn.eq_1, = Option.map_none, = Option.getD_none,
+    = Var.offsetOutNamed.eq_1, #f010]
+
+@[grind =, simp]
+theorem var_subst_neq
+{v : Var'}
+(h_neq : v ≠ x)
+: v.subst x r = (v↓x).get! := by
+  -- By the definition of subst, we just need to show it's not none
+  show (v↓x |>.map var |>.getD r) = (v↓x).get!
+  suffices v↓x ≠ none by
+    have : ∃ v', v↓x = some v' := Option.ne_none_iff_exists'.mp this
+    grind only [= id.eq_1, = Option.get!_some, = Option.map_some, = Option.getD_some, #4c12]
+  -- We need to treat each case differently sadly
+  cases varKind
+  · simp only [Var.offsetOut.simp_notation, Var.offsetOut, Var.offsetOutDeBruijn, Var.toNat,
+    gt_iff_lt, ne_eq, ite_eq_left_iff, not_imp]
+    grind only
+  · simp [Var.offsetOutNamed]
+    if h_name : v.name = x.name then
+      have h_depth: v.depth ≠ x.depth := by grind only [NamedVar.ext]
+      simp [h_name, h_depth]
+      grind only [→ eq_prop_or_type_of_isSort, = Option.map_some, = Option.getD_some, #baf6]
+    else
+      simp [h_name]
+
+@[grind =, simp]
+theorem subst_var_eq : x[x:=a] = a := by simp [Term.subst]
+
+@[grind =, simp]
+theorem subst_var_neq (h : x ≠ y)
+    : x[y:=a] = (x↓y).get (by exact Var.offsetOut_isSome_of_neq h) := by
+  grind only [Term.subst, = var_subst_neq, usr Var.offsetOut_eq_some_of_neq, = Option.get!_some,
+    = Option.get_some, #4d66]
+
+@[grind =, simp]
+theorem subst_sort : s[x:=a] = s := by
+  cases s using isSort_cases
+  all_goals rfl
+
+@[grind =, simp]
+theorem subst_of_not_mem_freeVars
+    (h_not_mem : x ∉ a.freeVars)
+    : a[x:=b] = (a↓x).get! := by
+  induction a
+  iterate 2 next => simp only [subst_sort, Term.offsetOut_sort, Option.get!_some] -- prop | type
+  case var v =>
+    change x ∉ [v] at h_not_mem
+    have : x ≠ v := by simpa using h_not_mem
+    rw [subst_var_neq this.symm]
+    rw [Term.offsetOut_var]
+    grind only [usr Var.offsetOut_eq_some_of_neq, = Option.map_some, = Option.get_some,
+      = Option.get!_some, #f94d]
+  case app f arg ih_f ih_arg =>
+    unfold Term.subst
+    rw [ih_f, ih_arg]
+    simp only [Term.offsetOut_app]
+    grind
+    sorry
+
+theorem subst_eq_sort [IsSort s]
+(h : a[x:=b] = s)
+: a = s ∨ (a = x ∧ b = s) := by
+  cases a <;> unfold Term.subst at h
+  -- prop | type
+  iterate 2 exact .inl assumption
+  -- main case
+  case var v =>
+    if h_v : v = x then
+      -- Replaced! that means b was it
+      right; show var v = x ∧ b = s
+      grind only [= var_subst_eq, = id.eq_1]
+    else
+      -- Not replaced! that means it was already s
+      left; show v = s
+      simp only [ne_eq, h_v, not_false_eq_true, var_subst_neq, Var.offsetOut.simp_notation] at h
+      grind only [→ eq_prop_or_type_of_isSort]
+  -- rest is candy
+  all_goals
+    cases s using isSort_cases
+    all_goals contradiction
+
+theorem double_subst
+    (h_x_neq_y : x ≠ y)
+    (h_not_mem : y ∉ a.freeVars)
+    : t[y:=b][(x↓y).get!:=a] = t[x:=a][y:=b[x:=a]] := by
+  induction t
+  iterate 2 next => simp only [subst_sort] -- prop | sort
+  case var z =>
+    apply distinguish z x y h_x_neq_y <;> intro h₁ h₂ ; subst_vars
+    case eq_x =>
+      simp [h_x_neq_y]
+      simp_all
+      rw [subst_var_neq, subst_var_eq]
+      simp
+
+    case x =>
+    · subst y z
+      simp
+    if h_x : z = x then
+      subst z
+      simp
+      if h_y : x = y then
+        subst y
+        simp
+      else
+        done
+      simp
+      
+    else
+      done
+  all_goals grind [Term.subst]
+  case app f arg ih_f ih_arg => grind [Term.subst]
+where
+  distinguish {α} [DecidableEq α]
+      (z x y : α) (h_x_neq_y : x ≠ y)
+      {motive : Prop}
+      (eq_x : z = x → z ≠ y → motive)
+      (eq_y : z = y → z ≠ x → motive)
+      (neither  : z ≠ x → z ≠ y → motive)
+      : motive := by
+    by_cases h₁ : z = x <;> by_cases h₂ : z = y
+    all_goals grind only
