Jrlean/Coc/VarDecl.lean
@@ -2,31 +2,41 @@ module
 
 public import Jrlean.Coc.VarKind
 
-import Jrlean.InstanceInfer
-
 namespace Jrlean.Coc
 
-public section
+@[expose] public section
 
+set_option linter.unusedVariables false in
 /-- The type of data that's needed to declare a variable of a given kind. -/
-abbrev VarDecl : [VarKind] → Type
+@[grind]
+def VarDecl : {varKind : VarKind} → Type
   | .deBruijn => Unit
   | .named => Lean.Name
 
 variable {varKind : VarKind}
 
 instance : Inhabited Lean.Name where default := `_
-instance : Inhabited VarDecl infer
-instance : DecidableEq VarDecl infer
-instance : Repr VarDecl infer
-instance : Hashable VarDecl infer
+local macro "infer " "instance " ": " typeClass:term : command => `(
+  instance : $typeClass (@VarDecl varKind) := by
+    unfold VarDecl
+    cases varKind <;> (
+      simp only
+      infer_instance
+    )
+)
+infer instance : Inhabited
+infer instance : DecidableEq
+infer instance : Repr
+infer instance : Hashable
+
+/-- A version of `VarDecl` that infers the variable kind via type-class inference. -/
+abbrev VarDecl' [VarKind] := @VarDecl inferInstance
 
 /--
 This returns a name to be used only for anonymous variables. Note that the variable can be accessed,
 they just shouldn't be.
 -/
-abbrev VarDecl.anonymous : VarDecl :=
+abbrev VarDecl.anonymous : VarDecl' :=
   match varKind with
   | .deBruijn => ()
   | .named => `_
-
